看一个简单的例子:
$$\begin{cases}x_1+x_2+x_3=6&{(1)}\\x_1+3x_2-2x_3=1&{(2)}\\2x_1-2x_2+x_3=1& {(3)}\end{cases}$$

 解：
 先用方程 (1) 消去方程 ${(3)}$ 中的 $x_{1}$ 
 即 $(2) - (1),(3)-2(1)$, 得到:
 $$\begin{cases}x_1+x_2+x_3=6&{(1)}\\2x_2-3x_3=-5&{(4)}\\-4x_2-x_3=-21&{(5)}\end{cases}$$
再 $(5)+2(4)$ 得同解三角方程组:
$$\left\{\begin{matrix}x_1+x_2+x_3=6\\2x_2-3x_3=-5\\-7x_3=-21\end{matrix}\right.$$
回代消元得到:
$$x_3=3,x_2=2,x_1=1$$

相当于:
**$$[A|b]=\begin{bmatrix}1&1&1&6\\[0.3em]1&3&-2&1\\[0.3em]2&-2&1&1\end{bmatrix}$$

化为:
$$\begin{bmatrix}1&1&1&6\\0&2&-3&-5\\0&-4&-1&-11\end{bmatrix}$$
再化为:
$$\begin{bmatrix}1&1&1&6\\0&2&-3&-5\\0&0&-7&-21\end{bmatrix}$$